coq/Modal_Tactics.v
@@ -7,6 +7,28 @@ Section Tactics.
 
 Context `{X: modal_index_set}.
 
+Lemma derive_identity:
+  forall A Γ φ,
+  Subset P A ->
+  A; Γ |-- [! φ -> φ !].
+Proof.
+  intros.
+  apply Mp with (f := [! φ -> φ -> φ !]).
+  - apply Mp with (f := [! φ -> (φ -> φ) -> φ !]).
+    + apply Ax with (a := ax2 φ [! φ -> φ !] φ).
+      * apply H.
+        constructor.
+      * reflexivity.
+    + apply Ax with (a := ax1 φ [! φ -> φ !]).
+      * apply H.
+        constructor.
+      * reflexivity.
+  - apply Ax with (a := ax1 φ φ).
+    + apply H.
+      constructor.
+    + reflexivity.
+Qed.
+
 Lemma deduction_subset:
   forall A G1 G2,
   Subset G1 G2 ->
